lib/coq/State_lemmas.v
@@ -658,7 +658,6 @@ Lemma liftState_read_memt Regs Regval A E rk a sz H r :
 unfold read_memt, read_memt_bytes, read_memtS, maybe_failS. simpl.
 apply bindS_cong; auto.
 intros [byte bit].
-replace_ArithFact_proof.
 destruct (of_bits _); auto.
 Qed.
 #[export] Hint Rewrite liftState_read_memt : liftState.
@@ -674,7 +673,6 @@ intros [ bytes | ]; auto. simpl.
 apply bindS_cong; auto.
 intros [byte bit].
 rewrite bindS_returnS_left. rewrite_liftState.
-replace_ArithFact_proof.
 destruct (of_bits _); auto.
 Qed.
 #[export] Hint Rewrite liftState_read_mem : liftState.
